feat: (1.1) fix reconstruct

Project 1/Ex1.dfy
@@ -34,20 +34,23 @@ function Deserialize(cs : seq<code>) : seq<aexpr>
 
 function reconstruct(cs : seq<code>, aes : seq<aexpr>) : seq<aexpr>
 	decreases cs, aes
-	requires forall k : int :: 0 <= k < cs.Length && cs[k].UnOpCode? 
-	 ==> aes.Length > 0 // TODO idk if this works or necessary TODO
-	requires forall k : int :: 0 <= k < cs.Length && cs[k].BinOpCode? 
-	 ==> aes.Length > 1 // TODO possibly not necessary
 {
 	if (cs == [])
 	then aes
-	else
-		match cs[0] {
-			case VarCode(s) => reconstruct(cs[1..], [Var(s)] + aes)
-			case ValCode(i) => reconstruct(cs[1..], [Val(i)] + aes)
-			case UnOpCode(op) => reconstruct(cs[1..], [UnOp(op, aes[0])] + aes[1..])
-			case BinOpCode(op) => reconstruct(cs[1..], [BinOp(op, aes[0], aes[1])] + aes[2..])
-		}
+	else reconstruct(cs[1..], reconstructAux(cs[0], aes))
+}
+
+function reconstructAux (cd : code, aes: seq<aexpr>) : seq<aexpr> {
+  match cd {
+    case VarCode(s) => [Var(s)] + aes
+	case ValCode(i) => [Val(i)] + aes
+	case UnOpCode(op) =>
+		if |aes| < 1 then [ ]
+		else [ UnOp(op, aes[0]) ] + aes[1..]
+	case BinOpCode(op) =>
+		if |aes| < 2 then [ ]
+		else [ BinOp(op, aes[1], aes[0]) ] + aes[2..]
+  }
 }
 
 
@@ -57,117 +60,126 @@ function reconstruct(cs : seq<code>, aes : seq<aexpr>) : seq<aexpr>
 lemma DeserializeProperty(e : aexpr)
   ensures Deserialize(Serialize(e)) == [ e ]
 {
-	calc {
-		Deserialize(Serialize(e));
-		== { deserializePropertyAux(e, [], []); }
-	}
-}
-
-lemma deserializePropertyAux(e : aexpr, cs : seq<code>, aes : seq<aexpr>)
-	ensures reconstruct(Serialize(e) + cs, ts) == reconstruct(cs, [e] + ts)
-	// ensures Deserialize(Serialize(e)+cs) == Deserialize(cs) + [e] // idk if this is preferable
-{
 	match e {
-		// base case??
 		case Var(s) => 
-		 calc {
-			reconstruct(Serialize(e) + cs, ts);
-			==
-			reconstruct(Serialize(Var(s)) + cs, ts); // by case
-			==
-			reconstruct([VarCode(s)] + cs, ts); // by def of Serialize
-			==
-			reconstruct(cs, [Var(s)] + ts); // by def of reconstruct
-			==
-			reconstruct(cs, [e] + ts); // by case
-		 }
-		case Val(i) =>
-		 calc {
-			reconstruct(Serialize(e) + cs, ts);
-			==
-			reconstruct(Serialize(Val(i)) + cs, ts); // by case
-			==
-			reconstruct([ValCode(i)] + cs, ts); // by def of Serialize
-			==
-			reconstruct(cs, [Val(i)] + ts); // by def of reconstruct
-			==
-			reconstruct(cs, [e] + ts); // by case
-		 }
-		// induction case
-		case UnOp(op, expr) =>
-		 // assert?
-		 calc {
-			reconstruct(Serialize(e) + cs, ts);
-			==
-			reconstruct(Serialize(UnOp(op, expr)) + cs, ts); // by case
-			==
-			reconstruct(Serialize(expr) + [UnOpCode(op)] + cs, ts); // def Serialize
-			== { deserializePropertyAux(expr, [UnOpCode(op)]+cs, ts); }
-			reconstruct([UnOpCode(op)] + cs, [expr] + ts); // IH
-			==
-			reconstruct(cs, [UnOp(op, expr)] + ts); // def reconstruct
-			==
-			reconstruct(cs, [e] + ts); // case
-		 }
-		case BinOp(op, expr1, expr2) =>
-		 assert [expr1] + ([expr2] + ts) == [expr1, expr2] + ts;
-		 calc {
-			reconstruct(Serialize(e) + cs, ts);
-			==
-			reconstruct(Serialize(BinOp(op, expr1, expr2)) + cs, ts); // by case
-			==
-			reconstruct(Serialize(expr2) + Serialize(expr1) + [BinOpCode(op)] + cs, ts); // def Serialize
-			== { deserializePropertyAux(expr2, (Serialize(expr1)+[BinOpCode(op)]+cs), ts); }
-			reconstruct(Serialize(expr1) + [BinOpCode(op)] + cs, [expr2] + ts); // IH
-			== { deserializePropertyAux(expr1, [BinOpCode(op)]+cs, [expr2] + ts); }
-			reconstruct([BinOpCode(op)] + cs, [expr1] + ([expr2] + ts)); // IH
-			==
-			reconstruct([BinOpCode(op)] + cs, [expr1, expr2] + ts); // properties of sequences
-			==
-			reconstruct(cs, [BinOp(op, expr1, expr2)] + ts); // def reconstruct
-			==
-			reconstruct(cs, [e] + ts); // case
-		 }
+			calc {
+				Deserialize(Serialize(e));
+				== // by case
+				Deserialize(Serialize(Var(s)));
+				== // by def of Serialize
+				Deserialize([VarCode(s)]);
+				== // unfolding Deserialize definition
+				reconstruct([VarCode(s)], []);
+				== // unfolding reconstruct definition
+				reconstruct([], [Var(s)] + []);
+				== // properties of sequences
+				reconstruct([], [Var(s)]);
+				== // defintion of reconstruct
+				[Var(s)];
+				== // by case
+				[e];
+			}
 	}
 }
 
-/*
-  Ex1.3
-*/
-function SerializeCodes(cs : seq<code>) : seq<nat> 
-{
+lemma ReconstructAfterSerializingLemma (t : aexpr, cds : seq<code>, ts : seq<aexpr>) 
+  ensures reconstruct(Serialize(t)+cds, ts) == reconstruct(cds, [ t ] + ts) {
 
+	match t {
+		case Var(s) => 
+			calc {
+				reconstruct(Serialize(t)+cds, ts);
+				== // by case
+				reconstruct(Serialize(Var(s))+cds, ts);
+				== // by unfolding def of Serialize
+				reconstruct([VarCode(s)]+cds, ts);
+				== // by unfolding def of reconstruct
+				reconstruct(cds, [Var(s)]+ts);
+				== // by case
+				reconstruct(cds, [t]+ts);
+			}
+		case Val(i) =>
+			calc {
+				reconstruct(Serialize(t)+cds, ts);
+				== // by case
+				reconstruct(Serialize(Val(i))+cds, ts);
+				== // by unfolding def of Serialize
+				reconstruct([ValCode(i)]+cds, ts);
+				== // by unfolding def of reconstruct
+				reconstruct(cds, [Val(i)]+ts);
+				== // by case
+				reconstruct(cds, [t]+ts);
+			}
+		case UnOp(op, expr) =>
+			calc {
+				reconstruct(Serialize(t)+cds, ts);
+				== // by case
+				reconstruct(Serialize(UnOp(op, expr)) + cds, ts);
+				== // by unfolding def of Serialize
+				reconstruct(Serialize(expr) + [UnOpCode(op)] + cds, ts);
+				//==
+			}
+		case BinOp(op, expr1, expr2) =>
+		    assert Serialize(expr2) + Serialize(expr1) + [ BinOpCode(op) ] + cds == Serialize(expr2) + (Serialize(expr1) + [ BinOpCode(op) ] + cds);
+			assert Serialize(expr1) + [BinOpCode(op)] + cds == Serialize(expr1) + ([BinOpCode(op)] + cds); 
+			assert  [ expr1 ] + ([ expr2 ] + ts) == [ expr1, expr2] + ts;
+			calc {
+				reconstruct(Serialize(t)+cds, ts);
+				== // by case
+				reconstruct(Serialize(BinOp(op, expr1, expr2)) + cds, ts);
+				== // by unfolding def of Serialize
+				reconstruct(Serialize(expr2) + Serialize(expr1) + [BinOpCode(op)] + cds, ts);
+				== { ReconstructAfterSerializingLemma(expr2, Serialize(expr1) + [BinOpCode(op)] + cds, ts); }
+				reconstruct(Serialize(expr1) + [BinOpCode(op)] + cds, [expr2] + ts);
+				== { ReconstructAfterSerializingLemma(expr1, [BinOpCode(op)] + cds, [expr2] + ts); }
+				reconstruct([BinOpCode(op)] + cds, [expr1] + ([expr2] + ts));
+				== // properties of sequences
+				reconstruct([BinOpCode(op)] + cds, [expr1, expr2] + ts);
+				== // by unfolding def of reconstruct
+				reconstruct(cds, [BinOp(op, expr1, expr2)] + ts);
+				== // by case
+				reconstruct(cds, [t] + ts);
+			}
+	}
 }
 
-function DeserializeCodes(ints : seq<nat>) : seq<code> {
+// /*
+//   Ex1.3
+// */
+// function SerializeCodes(cs : seq<code>) : seq<nat> 
+// {
+
+// }
+
+// function DeserializeCodes(ints : seq<nat>) : seq<code> {
   
-}
+// }
 
 
-/*
-  Ex1.4
-*/
-lemma DeserializeCodesProperty(cs : seq<code>)
-  ensures DeserializeCodes(SerializeCodes(cs)) == cs
-{
-}
+// /*
+//   Ex1.4
+// */
+// lemma DeserializeCodesProperty(cs : seq<code>)
+//   ensures DeserializeCodes(SerializeCodes(cs)) == cs
+// {
+// }
 
-/*
-  Ex1.5
-*/
-function FullSerialize(e : aexpr) : seq<nat> {
+// /*
+//   Ex1.5
+// */
+// function FullSerialize(e : aexpr) : seq<nat> {
  
-}
+// }
 
-function FullDeserealize(nats : seq<nat>) : seq<aexpr> {
+// function FullDeserealize(nats : seq<nat>) : seq<aexpr> {
  
-}
+// }
 
-/*
-  Ex1.6
-*/
-lemma FullDeserealizeProperty(e : aexpr)
-  ensures FullDeserealize(FullSerialize(e)) == [ e ]
-{
+// /*
+//   Ex1.6
+// */
+// lemma FullDeserealizeProperty(e : aexpr)
+//   ensures FullDeserealize(FullSerialize(e)) == [ e ]
+// {
     
-}
+// }
